Uniswap_Pool.thy
@@ -4,49 +4,49 @@ begin
 
 no_notation Reals ("\<real>") (*TODO: use that patch!*)
 
-type_synonym fee_protocal = \<open>nat \<times> nat\<close>
+type_synonym fee_protocol = \<open>nat \<times> nat\<close>
 
 datatype pool = pool (price: real) (tick: int) (unlocked: bool) (liquidity: real)
-                     (fee_growth_0: real) (fee_growth_1: real) (fee_protocal: fee_protocal)
+                     (growth: growth) (fee_protocol: fee_protocol) (protocal_fees: \<open>fee \<times> fee\<close>)
 
-hide_const (open) price tick unlocked liquidity fee_growth_0 fee_growth_1 fee_protocal
+hide_const (open) price tick unlocked liquidity growth fee_protocol protocal_fees
 
 setup \<open>Sign.mandatory_path "pool"\<close>
 
-definition \<open>map_price f x = (case x of pool p t u l f1 f2 fp \<Rightarrow> pool (f p) t u l f1 f2 fp)\<close>
+definition \<open>map_price f x = (case x of pool p t u l gr fp pf \<Rightarrow> pool (f p) t u l gr fp pf)\<close>
 lemma map_price[simp]:
-  \<open>pool.map_price f (pool p t u l f1 f2 fp) = pool (f p) t u l f1 f2 fp\<close>
+  \<open>pool.map_price f (pool p t u l gr fp pf) = pool (f p) t u l gr fp pf\<close>
   unfolding pool.map_price_def by simp
 
-definition \<open>map_tick f x = (case x of pool p t u l f1 f2 fp \<Rightarrow> pool p (f t) u l f1 f2 fp)\<close>
+definition \<open>map_tick f x = (case x of pool p t u l gr fp pf \<Rightarrow> pool p (f t) u l gr fp pf)\<close>
 lemma map_tick[simp]:
-  \<open>pool.map_tick f (pool p t u l f1 f2 fp) = pool p (f t) u l f1 f2 fp\<close>
+  \<open>pool.map_tick f (pool p t u l gr fp pf) = pool p (f t) u l gr fp pf\<close>
   unfolding pool.map_tick_def by simp
 
-definition \<open>map_unlock f x = (case x of pool p t u l f1 f2 fp \<Rightarrow> pool p t (f u) l f1 f2 fp)\<close>
+definition \<open>map_unlock f x = (case x of pool p t u l gr fp pf \<Rightarrow> pool p t (f u) l gr fp pf)\<close>
 lemma map_unlock[simp]:
-  \<open>pool.map_unlock f (pool p t u l f1 f2 fp) = pool p t (f u) l f1 f2 fp\<close>
+  \<open>pool.map_unlock f (pool p t u l gr fp pf) = pool p t (f u) l gr fp pf\<close>
   unfolding pool.map_unlock_def by simp
 
-definition \<open>map_liquidity f x = (case x of pool p t u l f1 f2 fp \<Rightarrow> pool p t u (f l) f1 f2 fp)\<close>
+definition \<open>map_liquidity f x = (case x of pool p t u l gr fp pf \<Rightarrow> pool p t u (f l) gr fp pf)\<close>
 lemma map_liquidity[simp]:
-  \<open>pool.map_liquidity f (pool p t u l f1 f2 fp) = pool p t u (f l) f1 f2 fp\<close>
+  \<open>pool.map_liquidity f (pool p t u l gr fp pf) = pool p t u (f l) gr fp pf\<close>
   unfolding pool.map_liquidity_def by simp
 
-definition \<open>map_fee_growth_0 f x = (case x of pool p t u l f1 f2 fp \<Rightarrow> pool p t u l (f f1) f2 fp)\<close>
-lemma fee_growth_0[simp]:
-  \<open>pool.map_fee_growth_0 f (pool p t u l f1 f2 fp) = pool p t u l (f f1) f2 fp\<close>
-  unfolding pool.map_fee_growth_0_def by simp
+definition \<open>map_growth f x = (case x of pool p t u l gr fp pf \<Rightarrow> pool p t u l (f gr) fp pf)\<close>
+lemma map_growth[simp]:
+  \<open>pool.map_growth f (pool p t u l gr fp pf) = pool p t u l (f gr) fp pf\<close>
+  unfolding pool.map_growth_def by simp
 
-definition \<open>map_fee_growth_1 f x = (case x of pool p t u l f1 f2 fp \<Rightarrow> pool p t u l f1 (f f2) fp)\<close>
-lemma map_fee_growth_1[simp]:
-  \<open>pool.map_fee_growth_1 f (pool p t u l f1 f2 fp) = pool p t u l f1 (f f2) fp\<close>
-  unfolding pool.map_fee_growth_1_def by simp
+definition \<open>map_fee_protocol f x = (case x of pool p t u l gr fp pf \<Rightarrow> pool p t u l gr (f fp) pf)\<close>
+lemma map_fee_protocol[simp]:
+  \<open>pool.map_fee_protocol f (pool p t u l gr fp pf) = pool p t u l gr (f fp) pf\<close>
+  unfolding pool.map_fee_protocol_def by simp
 
-definition \<open>map_fee_protocal f x = (case x of pool p t u l f1 f2 fp \<Rightarrow> pool p t u l f1 f2 (f fp))\<close>
-lemma map_fee_protocal[simp]:
-  \<open>pool.map_fee_protocal f (pool p t u l f1 f2 fp) = pool p t u l f1 f2 (f fp)\<close>
-  unfolding pool.map_fee_protocal_def by simp
+definition \<open>map_protocal_fees f x = (case x of pool p t u l gr fp pf \<Rightarrow> pool p t u l gr fp (f pf))\<close>
+lemma map_protocal_fees[simp]:
+  \<open>pool.map_protocal_fees f (pool p t u l gr fp pf) = pool p t u l gr fp (f pf)\<close>
+  unfolding pool.map_protocal_fees_def by simp
 
 setup \<open>Sign.parent_path\<close>
 
@@ -74,8 +74,12 @@ locale Pool = Tickmap_spec + Tick_spec +
     and op_set_fee_growth_0 :: \<open>(VAL,unit) proc'\<close>
     and op_get_fee_growth_1 :: \<open>VAL proc\<close>
     and op_set_fee_growth_1 :: \<open>(VAL,unit) proc'\<close>
-    and op_get_fee_protocal_0 :: \<open>VAL proc\<close>
-    and op_get_fee_protocal_1 :: \<open>VAL proc\<close>
+    and op_get_fee_protocol_0 :: \<open>VAL proc\<close>
+    and op_get_fee_protocol_1 :: \<open>VAL proc\<close>
+    and op_get_protocal_fee_0 :: \<open>VAL proc\<close>
+    and op_set_protocal_fee_0 :: \<open>(VAL,unit) proc'\<close>
+    and op_get_protocal_fee_1 :: \<open>VAL proc\<close>
+    and op_set_protocal_fee_1 :: \<open>(VAL,unit) proc'\<close>
   assumes [\<phi>inhabitance_rule]:
     \<open>s \<Ztypecolon> Pool \<i>\<m>\<p>\<l>\<i>\<e>\<s> UNIV \<a>\<n>\<d> 0 < pool.price s \<and> pool.tick s \<in> {MIN_TICK..<MAX_TICK}
                            \<and> pool.price s \<in> {MIN_PRICE..<MAX_PRICE}\<close>
@@ -96,28 +100,34 @@ locale Pool = Tickmap_spec + Tick_spec +
   and set_pool_liquidity_\<phi>app:
     \<open> \<p>\<r>\<o>\<c> op_set_liquidity rv \<lbrace> s \<Ztypecolon> Pool\<heavy_comma> l' \<Ztypecolon> \<v>\<a>\<l>[rv] \<real> \<longmapsto> pool.map_liquidity (\<lambda>_. l') s \<Ztypecolon> Pool \<rbrace> \<close>
   and get_pool_fee_growth_0_\<phi>app[\<phi>synthesis 1000]:
-    \<open> \<p>\<r>\<o>\<c> op_get_fee_growth_0 \<lbrace> s \<Ztypecolon> Pool \<longmapsto> s \<Ztypecolon> Pool\<heavy_comma> pool.fee_growth_0 s \<Ztypecolon> \<v>\<a>\<l> \<real> \<rbrace> \<close>
+    \<open> \<p>\<r>\<o>\<c> op_get_fee_growth_0 \<lbrace> s \<Ztypecolon> Pool \<longmapsto> s \<Ztypecolon> Pool\<heavy_comma> growth.fee0 (pool.growth s) \<Ztypecolon> \<v>\<a>\<l> \<real> \<rbrace> \<close>
   and set_pool_fee_growth_0_\<phi>app:
-    \<open> \<p>\<r>\<o>\<c> op_set_fee_growth_0 rv \<lbrace> s \<Ztypecolon> Pool\<heavy_comma> c' \<Ztypecolon> \<v>\<a>\<l>[rv] \<real> \<longmapsto> pool.map_fee_growth_0 (\<lambda>_. c') s \<Ztypecolon> Pool \<rbrace> \<close>
+    \<open> \<p>\<r>\<o>\<c> op_set_fee_growth_0 rv \<lbrace> s \<Ztypecolon> Pool\<heavy_comma> c' \<Ztypecolon> \<v>\<a>\<l>[rv] \<real> \<longmapsto> pool.map_growth (growth.map_fee0 (\<lambda>_. c')) s \<Ztypecolon> Pool \<rbrace> \<close>
   and get_pool_fee_growth_1_\<phi>app[\<phi>synthesis 1000]:
-    \<open> \<p>\<r>\<o>\<c> op_get_fee_growth_1 \<lbrace> s \<Ztypecolon> Pool \<longmapsto> s \<Ztypecolon> Pool\<heavy_comma> pool.fee_growth_1 s \<Ztypecolon> \<v>\<a>\<l> \<real> \<rbrace> \<close>
+    \<open> \<p>\<r>\<o>\<c> op_get_fee_growth_1 \<lbrace> s \<Ztypecolon> Pool \<longmapsto> s \<Ztypecolon> Pool\<heavy_comma> growth.fee1 (pool.growth s) \<Ztypecolon> \<v>\<a>\<l> \<real> \<rbrace> \<close>
   and set_pool_fee_growth_1_\<phi>app:
-    \<open> \<p>\<r>\<o>\<c> op_set_fee_growth_1 rv \<lbrace> s \<Ztypecolon> Pool\<heavy_comma> c' \<Ztypecolon> \<v>\<a>\<l>[rv] \<real> \<longmapsto> pool.map_fee_growth_1 (\<lambda>_. c') s \<Ztypecolon> Pool \<rbrace> \<close>
-  and get_fee_protocal_0[\<phi>synthesis 1000]:
-    \<open> \<p>\<r>\<o>\<c> op_get_fee_protocal_0 \<lbrace> s \<Ztypecolon> Pool \<longmapsto> s \<Ztypecolon> Pool\<heavy_comma> fst (pool.fee_protocal s) \<Ztypecolon> \<v>\<a>\<l> \<nat> \<rbrace> \<close>
-  and get_fee_protocal_1[\<phi>synthesis 1000]:
-    \<open> \<p>\<r>\<o>\<c> op_get_fee_protocal_1 \<lbrace> s \<Ztypecolon> Pool \<longmapsto> s \<Ztypecolon> Pool\<heavy_comma> snd (pool.fee_protocal s) \<Ztypecolon> \<v>\<a>\<l> \<nat> \<rbrace> \<close>
-
+    \<open> \<p>\<r>\<o>\<c> op_set_fee_growth_1 rv \<lbrace> s \<Ztypecolon> Pool\<heavy_comma> c' \<Ztypecolon> \<v>\<a>\<l>[rv] \<real> \<longmapsto> pool.map_growth (growth.map_fee1 (\<lambda>_. c')) s \<Ztypecolon> Pool \<rbrace> \<close>
+  and get_fee_protocol_0[\<phi>synthesis 1000]:
+    \<open> \<p>\<r>\<o>\<c> op_get_fee_protocol_0 \<lbrace> s \<Ztypecolon> Pool \<longmapsto> s \<Ztypecolon> Pool\<heavy_comma> fst (pool.fee_protocol s) \<Ztypecolon> \<v>\<a>\<l> \<nat> \<rbrace> \<close>
+  and get_fee_protocol_1[\<phi>synthesis 1000]:
+    \<open> \<p>\<r>\<o>\<c> op_get_fee_protocol_1 \<lbrace> s \<Ztypecolon> Pool \<longmapsto> s \<Ztypecolon> Pool\<heavy_comma> snd (pool.fee_protocol s) \<Ztypecolon> \<v>\<a>\<l> \<nat> \<rbrace> \<close>
+  and get_pool_protocal_fee_0_\<phi>app[\<phi>synthesis 1000]:
+    \<open> \<p>\<r>\<o>\<c> op_get_protocal_fee_0 \<lbrace> s \<Ztypecolon> Pool \<longmapsto> s \<Ztypecolon> Pool\<heavy_comma> fst (pool.protocal_fees s) \<Ztypecolon> \<v>\<a>\<l> \<real> \<rbrace> \<close>
+  and set_pool_protocal_fee_0_\<phi>app:
+    \<open> \<p>\<r>\<o>\<c> op_set_protocal_fee_0 rv \<lbrace> s \<Ztypecolon> Pool\<heavy_comma> c' \<Ztypecolon> \<v>\<a>\<l>[rv] \<real> \<longmapsto> pool.map_protocal_fees (apfst (\<lambda>_. c')) s \<Ztypecolon> Pool \<rbrace> \<close>
+  and get_pool_protocal_fee_1_\<phi>app[\<phi>synthesis 1000]:
+    \<open> \<p>\<r>\<o>\<c> op_get_protocal_fee_1 \<lbrace> s \<Ztypecolon> Pool \<longmapsto> s \<Ztypecolon> Pool\<heavy_comma> snd (pool.protocal_fees s) \<Ztypecolon> \<v>\<a>\<l> \<real> \<rbrace> \<close>
+  and set_pool_protocal_fee_1_\<phi>app:
+    \<open> \<p>\<r>\<o>\<c> op_set_protocal_fee_1 rv \<lbrace> s \<Ztypecolon> Pool\<heavy_comma> c' \<Ztypecolon> \<v>\<a>\<l>[rv] \<real> \<longmapsto> pool.map_protocal_fees (apsnd (\<lambda>_. c')) s \<Ztypecolon> Pool \<rbrace> \<close>
 
 begin
 
-term growth.fee0
 
-definition Uniswap_Pool :: \<open>(fiction, real \<times> tick \<times> bool \<times> liquidity \<times> liquidity \<times> growths \<times> opt_growths \<times> fee_protocal) \<phi>\<close>
+definition Uniswap_Pool :: \<open>(fiction, price \<times> tick \<times> bool \<times> liquidity \<times> liquidity \<times> growths \<times> opt_growths \<times> fee_protocol \<times> (fee \<times> fee)) \<phi>\<close>
   where [\<phi>defs]: \<open>Uniswap_Pool x = (
-    case x of (price, i, unlocked, Lg, L, growth, \<delta>, fee_proto) \<Rightarrow>
+    case x of (price, i, unlocked, Lg, L, growth, \<delta>, fee_proto, protocal_fees) \<Rightarrow>
         \<comment> \<open>\<open>growth\<close> is the abstract growth happened on every tick\<close>
-      pool price i unlocked (L i) (growth.fee0 (gSum growth)) (growth.fee1 (gSum growth)) fee_proto \<Ztypecolon> Pool\<heavy_comma>
+      pool price i unlocked (L i) (gSum growth) fee_proto protocal_fees \<Ztypecolon> Pool\<heavy_comma>
         \<comment> \<open>so the global fee growth is the sum of the \<open>growth\<close> over every tick\<close>
       (\<lambda>k. 0 < Lg k) \<Ztypecolon> Tickmap\<heavy_comma>
         \<comment> \<open>\<open>k \<in> dom \<delta>\<close> means the tick \<open>k\<close> is initialized\<close>
@@ -128,8 +138,8 @@ definition Uniswap_Pool :: \<open>(fiction, real \<times> tick \<times> bool \<t
 declare [[\<phi>trace_reasoning = 1]]
 
 lemma [\<phi>reason 1200]:
-  \<open>(price, i, unlocked, Lg, L, growth, \<delta>, fee_proto) \<Ztypecolon> Uniswap_Pool \<i>\<m>\<p>\<l>\<i>\<e>\<s>
-   pool price i unlocked (L i) (growth.fee0 (gSum growth)) (growth.fee1 (gSum growth)) fee_proto \<Ztypecolon> Pool\<heavy_comma>
+  \<open>(price, i, unlocked, Lg, L, growth, \<delta>, fee_proto, protocal_fees) \<Ztypecolon> Uniswap_Pool \<i>\<m>\<p>\<l>\<i>\<e>\<s>
+   pool price i unlocked (L i) (gSum growth) fee_proto protocal_fees \<Ztypecolon> Pool\<heavy_comma>
    (\<lambda>k. 0 < Lg k) \<Ztypecolon> Tickmap\<heavy_comma>
    (Lg, L, growth, i, \<delta>) \<Ztypecolon> Ticks
   \<a>\<n>\<d> (tick_of_price price = i \<or> price = price_of (i + 1))
@@ -138,32 +148,70 @@ lemma [\<phi>reason 1200]:
 
 lemma [\<phi>reason 100]:
   \<open> \<p>\<r>\<e>\<m>\<i>\<s>\<e> (tick_of_price price = i \<or> price = price_of (i + 1))
-\<Longrightarrow> X \<i>\<m>\<p>\<l>\<i>\<e>\<s> pool price i unlocked (L i) (growth.fee0 (gSum growth)) (growth.fee1 (gSum growth)) fee_proto \<Ztypecolon> Pool\<heavy_comma>
+\<Longrightarrow> X \<i>\<m>\<p>\<l>\<i>\<e>\<s> pool price i unlocked (L i) (gSum growth) fee_proto protocal_fees \<Ztypecolon> Pool\<heavy_comma>
         (\<lambda>k. 0 < Lg k) \<Ztypecolon> Tickmap\<heavy_comma>
-        (Lg, L, growth, i, \<delta>) \<Ztypecolon> Ticks \<a>\<n>\<d> P
-\<Longrightarrow> X \<i>\<m>\<p>\<l>\<i>\<e>\<s> (price, i, unlocked, Lg, L, growth, \<delta>, fee_proto) \<Ztypecolon> Uniswap_Pool \<a>\<n>\<d> P\<close>
+        (Lg, L, growth, i, \<delta>) \<Ztypecolon> Ticks \<r>\<e>\<m>\<a>\<i>\<n>\<s> R \<a>\<n>\<d> P
+\<Longrightarrow> X \<i>\<m>\<p>\<l>\<i>\<e>\<s> (price, i, unlocked, Lg, L, growth, \<delta>, fee_proto, protocal_fees) \<Ztypecolon> Uniswap_Pool \<r>\<e>\<m>\<a>\<i>\<n>\<s> R \<a>\<n>\<d> P\<close>
+  unfolding FOCUS_TAG_def
   \<medium_left_bracket> premises _ and I
-    I construct\<phi> \<open>(price, i, unlocked, Lg, L, growth, \<delta>, fee_proto) \<Ztypecolon> Uniswap_Pool\<close> \<medium_right_bracket>. .
+    I 
+    construct\<phi> \<open>(price, i, unlocked, Lg, L, growth, \<delta>, fee_proto, protocal_fees) \<Ztypecolon> Uniswap_Pool\<close>
+  \<medium_right_bracket>. .
 
 declare Invt_Ticks_def[simp] Invt_A_Tick_def[simp]
 
 (*
 definition swap_loop_transition :: \<open>bool \<Rightarrow> bool \<Rightarrow> nat \<times> nat \<Rightarrow> liquidity \<Rightarrow> tick \<times> fee \<Rightarrow> unit\<close>
-  where \<open>swap_loop_transition exactIn zeroForOne fee_protocal L
+  where \<open>swap_loop_transition exactIn zeroForOne fee_protocol L
     =(\<lambda>(j,ar).
-      let fee_proto = (if zeroForOne then fst fee_protocal else snd fee_protocal) ;
+      let fee_proto = (if zeroForOne then fst fee_protocol else snd fee_protocol) ;
           (next_price, amountIn, amountOut, fee_amount) =
   swap_step pr (if zeroForOne then max (price_of tick_next) price_limit else min (price_of tick_next) price_limit) (L j) ar fee
        in ())\<close> *)
 
+definition \<open>\<Delta>protocal_fees fee_proto zeroForOne L price price' \<gamma>
+    = (if zeroForOne
+       then if 0 < fst fee_proto
+            then (fst (reserve_change zeroForOne L price price') * fee_factor / real (fst fee_proto), 0)
+            else (0,0)
+       else if 0 < snd fee_proto
+            then (0, snd (reserve_change zeroForOne L price price') * fee_factor / real (snd fee_proto))
+            else (0,0))\<close>
+
 proc swap:
-  input \<open>(price, i, unlocked, Lg, L, growth, \<delta>, fee_protocal) \<Ztypecolon> Uniswap_Pool\<heavy_comma>
+  input \<open>(price, i, unlocked, Lg, L, growth, \<delta>, fee_protocol, protocal_fees) \<Ztypecolon> Uniswap_Pool\<heavy_comma>
          recipient \<Ztypecolon> \<v>\<a>\<l> Address\<heavy_comma> zeroForOne \<Ztypecolon> \<v>\<a>\<l> \<bool>\<heavy_comma> amount_specified \<Ztypecolon> \<v>\<a>\<l> \<real>\<heavy_comma> price_limit \<Ztypecolon> \<v>\<a>\<l> \<real>\<close>
   premises \<open>0 \<noteq> amount_specified \<and> 0 < price_limit\<close> and \<open>unlocked\<close>
       and \<open>if zeroForOne then price_limit < price \<and> price_limit > MIN_PRICE
                          else price_limit > price \<and> price_limit < MAX_PRICE\<close>
-    (*soon we will have exception-based require statement*)
-  output \<open>amount0 \<Ztypecolon> \<v>\<a>\<l> \<real>\<heavy_comma> amount1 \<Ztypecolon> \<v>\<a>\<l> \<real>\<close>
+    (*soon we will not need to declare these pre-conditions but verify that
+        a revert will happen once they are violated*)
+  output \<open>(price', i', unlocked, Lg, L,
+            growth + fee_growth zeroForOne fee_factor L price price',
+            \<delta>, fee_protocol,
+            protocal_fees + \<Delta>protocal_fees fee_protocol zeroForOne L price price' fee_factor) \<Ztypecolon> Uniswap_Pool\<heavy_comma>
+          transfer_out \<Ztypecolon> \<v>\<a>\<l> \<real>\<heavy_comma> transfer_in \<Ztypecolon> \<v>\<a>\<l> \<real>
+    \<s>\<u>\<b>\<j> price' i' transfer_out transfer_in.
+      (if zeroForOne then price_limit \<le> price' else price' \<le> price_limit) \<and>
+      (price' = price_limit \<or> (
+      if 0 < amount_specified
+      then amount_specified * (1 - fee) = (if zeroForOne then fst else snd) (reserve_change zeroForOne L price price')
+      else - amount_specified = (if zeroForOne then snd else fst) (reserve_change zeroForOne L price price') ))
+      \<comment> \<open>The resulted price either reaches the price limit, or, is the one having a reserve change
+             meeting the specified amount.
+          \<open>reserve_change zeroForOne L price price'\<close> is the reserve change of token0 and token1
+             when the price is moving from \<open>price\<close> to \<open>price'\<close>\<close>
+      \<comment> \<open>The tick \<open>i'\<close> is the one satisfying the global invariant encoded in \<^const>\<open>Uniswap_Pool\<close>,
+          which is, \<open>i'\<close> is the tick of the \<open>price'\<close>, \<open>price_of i' \<le> price \<le> price_of (i' + 1)\<close>\<close>
+      \<comment> \<open>Gross liquidity \<open>Lg\<close>, actual liquidity \<open>L\<close>, the absolute difference \<open>\<delta>\<close> in recorded fee growth,
+          and the proportion \<open>fee_protocol\<close> of the protocol fee, are not changed\<close>
+      \<comment> \<open>The fee growth \<open>growth + fee_growth zeroForOne fee_factor L price price'\<close>
+          and the \<open>protocal_fees\<close> are increased accordingly.\<close>
+   \<and> transfer_out = (if zeroForOne then snd else fst) (reserve_change zeroForOne L price price')
+   \<and> transfer_in = (if zeroForOne then fst else snd) (reserve_change zeroForOne L price price') / (1 - fee)
+    \<comment> \<open>As \<phi>-system hasn't formalized transfer and external call, we cannot verify the last transfer operation
+      in the swap function, but only verify the amount of transfer-out and that of transfer-in. \<close>
+\<close>
   is [routine]
   (* is [noDelegateCall]  Currently no modifier is supported, but is planned *)
   \<medium_left_bracket> D ;;
@@ -175,10 +223,10 @@ proc swap:
             $zeroForOne)) ;;
     set_pool_unlock (\<open>False\<close>)  ;;
 
-    define fee_proto where \<open>fee_proto = (if zeroForOne then fst fee_protocal else snd fee_protocal)\<close> ;;
+    define fee_proto where \<open>fee_proto = (if zeroForOne then fst fee_protocol else snd fee_protocol)\<close> ;;
 
     \<open>pool.liquidity _\<close> \<rightarrow> val liquidityStart
-    sel (\<open>fst (pool.fee_protocal _)\<close> \<open>snd (pool.fee_protocal _)\<close> $zeroForOne)
+    sel (\<open>fst (pool.fee_protocol _)\<close> \<open>snd (pool.fee_protocol _)\<close> $zeroForOne)
         is fee_proto affirm unfolding fee_proto_def by simp ;; \<rightarrow> val feeProtocol
     \<open>0 \<Ztypecolon> \<real>\<close> \<rightarrow> val secondsPerLiquidityCumulative
     \<open>0 \<Ztypecolon> \<real>\<close> \<rightarrow> val tickCumulative
@@ -192,12 +240,12 @@ proc swap:
 
     $amount_specified, \<open>0 \<Ztypecolon> \<real>\<close>,
       \<open>pool.price _\<close>, \<open>pool.tick _\<close>,
-      sel (\<open>pool.fee_growth_0 _\<close> \<open>pool.fee_growth_1 _\<close> $zeroForOne)
+      sel (\<open>growth.fee0 (pool.growth _)\<close> \<open>growth.fee1 (pool.growth _)\<close> $zeroForOne)
           is \<open>I_fee_growth_global growth\<close> affirm unfolding I_fee_growth_global_def by simp ;;
       \<open>0 \<Ztypecolon> \<real>\<close>, $liquidityStart
-    \<rightarrow> var amount_reamining, amount_calculated, price, tick, fee_growth_global, protocolFee, liquidity ;;
+    \<rightarrow> var amount_remaining, amount_calculated, price, tick, fee_growth_global, protocolFee, liquidity ;;
 
-    while \<open>ar \<Ztypecolon> \<v>\<a>\<r>[\<v>\<a>\<r>_amount_reamining] \<real>\<heavy_comma>
+    while \<open>ar \<Ztypecolon> \<v>\<a>\<r>[\<v>\<a>\<r>_amount_remaining] \<real>\<heavy_comma>
            pr \<Ztypecolon> \<v>\<a>\<r>[\<v>\<a>\<r>_price] \<real>\<heavy_comma>
            ac \<Ztypecolon> \<v>\<a>\<r>[\<v>\<a>\<r>_amount_calculated] \<real>\<heavy_comma>
            pf \<Ztypecolon> \<v>\<a>\<r>[\<v>\<a>\<r>_protocolFee] \<real>\<heavy_comma>
@@ -210,7 +258,7 @@ proc swap:
                  \<and> j < MAX_TICK
                  \<and> (tick_of_price pr = j \<or> pr = price_of (j + 1))
                  \<and> (if zeroForOne then price_limit \<le> pr \<and> pr \<le> price else price \<le> pr \<and> pr \<le> price_limit)
-                 \<and> (let (\<Delta>reserve0, \<Delta>reserve1) = (if zeroForOne then reserve_change L pr price else reserve_change L price pr);
+                 \<and> (let (\<Delta>reserve0, \<Delta>reserve1) = reserve_change zeroForOne L price pr;
                         amountIn = (if zeroForOne then \<Delta>reserve0 else \<Delta>reserve1) ;
                         amountOut = (if zeroForOne then \<Delta>reserve1 else \<Delta>reserve0)
                      in (if ?exactInput then amount_specified - amountIn / (1 - fee) else amount_specified + amountOut) = ar
@@ -220,7 +268,7 @@ proc swap:
                  
           )
           \<and> Guard: (ar \<noteq> 0 \<and> pr \<noteq> price_limit)\<close>
-    \<medium_left_bracket> \<open>$amount_reamining \<noteq> 0 \<and> $price \<noteq> $price_limit\<close> \<medium_right_bracket>.
+    \<medium_left_bracket> \<open>$amount_remaining \<noteq> 0 \<and> $price \<noteq> $price_limit\<close> \<medium_right_bracket>.
     \<medium_left_bracket>
       $price \<rightarrow> val step_price_start ;;
       nextInitializedTickWithinOneWord ($tick, $zeroForOne) \<exists>tick_next' \<rightarrow> var tick_next, val initialized ;;
@@ -237,9 +285,7 @@ proc swap:
 
       have t2: \<open>0 < Lg tick_next' \<Longrightarrow> 0 < Lg tick_next\<close> by (smt (verit, ccfv_SIG) \<open>tick_next \<in> {MIN_TICK..MAX_TICK} \<and> (if tick_next' < MIN_TICK then MIN_TICK else if MAX_TICK < tick_next' then MAX_TICK else tick_next') = tick_next \<and> True\<close> the_\<phi>(18))
 
-      have tick_next_dom: \<open>MIN_TICK \<le> tick_next\<close> \<open>tick_next \<le> MAX_TICK\<close>
-        using the_\<phi>(4) apply force
-        using the_\<phi>(5) by blast
+      have tick_next_dom: \<open>MIN_TICK \<le> tick_next\<close> \<open>tick_next \<le> MAX_TICK\<close> using the_\<phi>(4) the_\<phi>(5) by blast+
 
       have y0: \<open>if j < tick_next' then next_initialized Lg j tick_next' else next_initialized Lg (tick_next') (j+1)\<close>
         by (auto,
@@ -254,8 +300,6 @@ proc swap:
       have x1': \<open>\<not> zeroForOne \<Longrightarrow> j < tick_next\<close> using the_\<phi>(27) the_\<phi>lemmata(4) tick_next_def by force
 
       have t8: \<open>zeroForOne \<Longrightarrow> \<forall>k. tick_next < k \<and> k \<le> j \<longrightarrow> Lg k = 0\<close> using y1 by force
-
-      have t8': \<open>\<not> zeroForOne \<Longrightarrow> \<forall>k. j < k \<and> k < tick_next \<longrightarrow> Lg k = 0\<close> using y1 by force
 
       have t8': \<open>\<not> zeroForOne \<Longrightarrow> \<forall>k. j < k \<and> k \<le> (tick_next - 1) \<longrightarrow> Lg k = 0\<close> using y1 by force
 
@@ -283,8 +327,9 @@ proc swap:
                 sel (\<open>$step_price_next < $price_limit\<close>, \<open>$step_price_next > $price_limit\<close>, $zeroForOne))
          is \<open>if zeroForOne then max ?step_price_next price_limit else min ?step_price_next price_limit\<close>,
         $liquidity,
-        $amount_reamining,
-        fee) \<exists>next_price, amountIn, amountOut, fee_amount
+        $amount_remaining,
+        fee)
+        \<exists>next_price, amountIn, amountOut, fee_amount
      \<rightarrow> val amountIn, amountOut, feeAmount \<rightarrow> price ;;
      (*FIX ME: ^ there is a bug*)
 
@@ -296,11 +341,9 @@ proc swap:
 
       have kk1: \<open>MIN_PRICE < (if zeroForOne then max ?step_price_next price_limit else min ?step_price_next price_limit)\<close> using price_of_smono the_\<phi>(24) the_\<phi>(27) the_\<phi>(31) the_\<phi>(33) the_\<phi>lemmata(2) x1' by force
 
-      have kk3: \<open>\<not> zeroForOne \<Longrightarrow> min ?step_price_next price_limit < MAX_PRICE\<close> using the_\<phi>(33) by force
-
       have kk2: \<open>MIN_PRICE < next_price\<close> using fee_range kk1 swap_step_next_price_Le_MIN_PRICE the_\<phi>(16) the_\<phi>(25) the_\<phi>(31) the_\<phi>lemmata(5) by blast
 
-      have kk4: \<open>\<not> zeroForOne \<Longrightarrow> next_price < MAX_PRICE\<close> by (smt (verit, ccfv_SIG) fee_range kk1 kk3 price_of_L0 swap_step_next_price_Gt_MAX t0 the_\<phi>(16) the_\<phi>(25) the_\<phi>(30) the_\<phi>lemmata(5))
+      have kk4: \<open>\<not> zeroForOne \<Longrightarrow> next_price < MAX_PRICE\<close> by (smt (verit, best) fee_range price_of_L0 swap_step_next_price_Gt t0 the_\<phi>(16) the_\<phi>(25) the_\<phi>(27) the_\<phi>(33) the_\<phi>lemmata(5))
         
       have kk8: \<open>zeroForOne \<Longrightarrow> next_price \<le> pr\<close> by (smt (verit, best) fee_range price_of_L0 price_of_smono price_of_tick swap_step_next_price_LE_price t0 the_\<phi>(16) the_\<phi>(27) the_\<phi>(28) the_\<phi>lemmata(5) x1) 
 
@@ -313,11 +356,9 @@ proc swap:
         apply (smt (verit, ccfv_threshold) fee_range kk9 price_of_L0 swap_step_next_price_Gt t0 the_\<phi>(16) the_\<phi>(25) the_\<phi>(27) the_\<phi>lemmata(5))
         by (smt (verit, ccfv_SIG) fee_range price_of_L0 swap_step_next_price_LE_price swap_step_next_price_LE_price_target t0 the_\<phi>(16) the_\<phi>(27) the_\<phi>lemmata(5))
 
-      have ka1: \<open>zeroForOne \<Longrightarrow> \<forall>k. tick_of_price next_price < k \<and> k < tick_of_price pr \<longrightarrow> Lg k = 0\<close>
-        by (metis dual_order.strict_trans2 kk6 order.strict_iff_not price_of_L0 t8 the_\<phi>(28) tick_of_price tick_of_price_LE_mono zle_add1_eq_le)
+      have ka1: \<open>zeroForOne \<Longrightarrow> \<forall>k. tick_of_price next_price < k \<and> k < tick_of_price pr \<longrightarrow> Lg k = 0\<close> by (metis dual_order.strict_trans2 kk6 order.strict_iff_not price_of_L0 t8 the_\<phi>(28) tick_of_price tick_of_price_LE_mono zle_add1_eq_le)
 
-      have ka2: \<open>\<not> zeroForOne \<Longrightarrow> \<forall>k. tick_of_price pr < k \<and> k < tick_of_price next_price \<longrightarrow> Lg k = 0\<close>
-        by (smt (verit, del_insts) kk2 kk7 price_of_L0 the_\<phi>(28) tick_of_price tick_of_price_LE_mono y1)
+      have ka2: \<open>\<not> zeroForOne \<Longrightarrow> \<forall>k. tick_of_price pr < k \<and> k < tick_of_price next_price \<longrightarrow> Lg k = 0\<close> by (smt (verit, del_insts) kk2 kk7 price_of_L0 the_\<phi>(28) tick_of_price tick_of_price_LE_mono y1)
 
       have kb1: \<open>zeroForOne \<Longrightarrow> \<forall>k. next_price \<le> k \<and> k < pr \<longrightarrow> L (tick_of_price k) = L j\<close>
         by (smt (verit) kk6 price_of_L0 price_of_tick t7 the_\<phi>(28) tick_of_price tick_of_price_LE_mono)
@@ -329,7 +370,7 @@ proc swap:
         by (smt (verit, ccfv_SIG) fee_range kk6 price_of_smono price_of_tick swap_step_next_price_Gt t7 the_\<phi>(16) the_\<phi>(19) the_\<phi>(24) the_\<phi>(25) the_\<phi>(27) the_\<phi>(28) the_\<phi>(35) x1)
 
       have p2: \<open>if zeroForOne then (amountIn, amountOut) = reserve_change_in_a_step (L (tick_of_price next_price)) next_price pr
-                          else (amountOut, amountIn) = reserve_change_in_a_step (L (tick_of_price pr)) pr next_price\<close>
+                              else (amountOut, amountIn) = reserve_change_in_a_step (L (tick_of_price pr)) pr next_price\<close>
         apply (cases zeroForOne; simp)
         apply (smt (verit, ccfv_SIG) kk6 kk8 p1 swap_step_reserve_change_zeroForOne the_\<phi>lemmata(5))
         by (smt (verit, ccfv_SIG) growth.fee0 growth.fee0.homo_zero growth.fee1 growth.fee1.homo_zero kk7 kk9 price_of_smono reserve_change_in_a_tick_0 swap_step_reserve_change_not_zeroForOne swap_step_reserve_change_zeroForOne t11 the_\<phi>(28) the_\<phi>lemmata(5) tick_of_price)
@@ -343,10 +384,10 @@ proc swap:
 
 
       if \<open>$exactInput\<close> \<medium_left_bracket>
-          \<open>$amount_reamining - ($amountIn + $feeAmount)\<close> \<rightarrow> amount_reamining
+          \<open>$amount_remaining - ($amountIn + $feeAmount)\<close> \<rightarrow> amount_remaining
           \<open>$amount_calculated - $amountOut\<close> \<rightarrow> amount_calculated
       \<medium_right_bracket>. \<medium_left_bracket>
-          \<open>$amount_reamining + $amountOut\<close> \<rightarrow> amount_reamining
+          \<open>$amount_remaining + $amountOut\<close> \<rightarrow> amount_remaining
           \<open>$amount_calculated + ($amountIn + $feeAmount)\<close> \<rightarrow> amount_calculated
       \<medium_right_bracket>. ;;
 
@@ -359,14 +400,6 @@ proc swap:
       define step_growth where \<open>step_growth = (if L j = 0 then 0 else fee_amount / L j)\<close>
       define \<Delta>growth where \<open>\<Delta>growth = fee_growth zeroForOne fee_factor L pr next_price\<close> 
 
-(*
-
-      grow_current_tick[where \<Delta>=\<open>if zeroForOne then (step_growth, 0) else (0, step_growth)\<close>]
-        affirm by (auto simp add: zero_prod_def, cases zeroForOne,
-                   smt (verit, best) divide_nonneg_nonneg fee_range local.step_growth_def price_of_L0 swap_step_fee_Le_0 t0 the_\<phi>(16) the_\<phi>lemmata(5),
-                   smt (verit, best) divide_nonneg_nonneg fee_range kk1 local.step_growth_def price_of_L0 swap_step_fee_Le_0 t0 the_\<phi>(16) the_\<phi>lemmata(5)) ;; ;;
-        is \<open>(Lg, L, growth' + \<Delta>growth, _, _)\<close> affirm unfolding \<Delta>growth_def step_growth_def by (simp add: plus_fun fun_eq_iff) auto *)
-      ;;
       have ak1: \<open>0 < L j \<Longrightarrow> zeroForOne \<Longrightarrow> global_fee0_growth (fee_growth' True fee_factor L next_price pr) = (1/next_price - 1/pr) * fee_factor\<close>
         using gSum_fee_growth kb1 kk2 kk8 the_\<phi>(30) by force
 
@@ -396,19 +429,17 @@ proc swap:
 
         if \<open>$initialized\<close> \<medium_left_bracket>
 
-        
-        ;;
            $tick_next,
 
-           sel ($fee_growth_global, \<open>pool.fee_growth_0 _\<close>, $zeroForOne)
+           sel ($fee_growth_global, \<open>growth.fee0 (pool.growth _)\<close>, $zeroForOne)
               is \<open>global_fee0_growth (?growth' + \<Delta>growth)\<close>
-            affirm unfolding I_fee_growth_global_def \<Delta>growth_def
-              by (auto simp add: zero_fun_def, insert fee_growth_is_0_when_not_zeroForOne kk9 the_\<phi>(1) the_\<phi>(29), force) ;;
+              affirm unfolding I_fee_growth_global_def \<Delta>growth_def
+                by (auto simp add: zero_fun_def, insert fee_growth_is_0_when_not_zeroForOne kk9 the_\<phi>(1) the_\<phi>(29), force) ;;
 
-           sel (\<open>pool.fee_growth_1 _\<close>, $fee_growth_global, $zeroForOne)
+           sel (\<open>growth.fee1 (pool.growth _)\<close>, $fee_growth_global, $zeroForOne)
               is \<open>global_fee1_growth (?growth' + \<Delta>growth)\<close>
-            affirm unfolding I_fee_growth_global_def \<Delta>growth_def
-              by (auto simp add: zero_fun_def) (smt (verit, ccfv_SIG) fee_growth_is_0_when_zeroForOne kk2 kk8 price_of_L0 the_\<phi>(29)) ;;
+              affirm unfolding I_fee_growth_global_def \<Delta>growth_def
+                by (auto simp add: zero_fun_def) (smt (verit, ccfv_SIG) fee_growth_is_0_when_zeroForOne kk2 kk8 price_of_L0 the_\<phi>(29)) ;;
            (*TODO: syntax*)
            tick_cross[where \<Delta>=\<Delta>growth]
               affirm using t2 the_\<phi>(19) by presburger ;;
@@ -488,17 +519,17 @@ proc swap:
         shift_current_tick_\<Delta>[where j=\<open>tick_of_price next_price\<close> and \<Delta>=\<Delta>growth]
           affirm using the_\<phi>(4) the_\<phi>(5) by fastforce ;;
           affirm using y1 zx1 zx2 zz6 zz7 by force ;;
-affirm unfolding \<Delta>growth_def real_next_tick_def apply auto
-  using fee_growth_eq_0 kk2 kk8 the_\<phi>(33) apply auto[1]
-  apply (smt (verit) fee_growth_eq_0 kk2 kk8 the_\<phi>(31) the_\<phi>(33) tick_of_price)
-  using zx1 apply blast
-  using zx1 apply fastforce
-  using fee_growth_eq_0 kk4 kk9 the_\<phi>(31) the_\<phi>(34) apply auto[1]
-  using fee_growth_eq_0 kk4 kk9 the_\<phi>(34) apply force
-  using fee_growth_eq_0 kk4 kk9 the_\<phi>(31) the_\<phi>(34) apply auto[1]
-  using fee_growth_eq_0 kk4 kk9 the_\<phi>(34) by blast ;;
-  affirm unfolding \<Delta>growth_def
-  using fee_factor_GT_0 fee_growth_always_ge_0 kk6 kk8 kk9 t0 the_\<phi>(38) by auto 
+          affirm unfolding \<Delta>growth_def real_next_tick_def apply auto
+              using fee_growth_eq_0 kk2 kk8 the_\<phi>(33) apply auto[1]
+              apply (smt (verit) fee_growth_eq_0 kk2 kk8 the_\<phi>(31) the_\<phi>(33) tick_of_price)
+              using zx1 apply blast
+              using zx1 apply fastforce
+              using fee_growth_eq_0 kk4 kk9 the_\<phi>(31) the_\<phi>(34) apply auto[1]
+              using fee_growth_eq_0 kk4 kk9 the_\<phi>(34) apply force
+              using fee_growth_eq_0 kk4 kk9 the_\<phi>(31) the_\<phi>(34) apply auto[1]
+              using fee_growth_eq_0 kk4 kk9 the_\<phi>(34) by blast ;;
+              affirm unfolding \<Delta>growth_def
+              using fee_factor_GT_0 fee_growth_always_ge_0 kk6 kk8 kk9 t0 the_\<phi>(38) by auto 
       \<medium_right_bracket>. ;;
 
       define real2_next_tick where
@@ -514,8 +545,7 @@ affirm unfolding \<Delta>growth_def real_next_tick_def apply auto
         using kk4 kk6 kk8 kk9 less_MAX_PRICE_less_MAX_TICK t0 the_\<phi>(24) the_\<phi>(29) by fastforce
              
 
-      have Iv2: \<open>MIN_PRICE \<le> next_price \<and> next_price < MAX_PRICE\<close>
-        using kk2 kk4 kk8 the_\<phi>(24) by force
+      have Iv2: \<open>MIN_PRICE \<le> next_price \<and> next_price < MAX_PRICE\<close> using kk2 kk4 kk8 the_\<phi>(24) by force
       
       have Iv3: \<open>tick_of_price next_price = real2_next_tick \<or> next_price = price_of (real2_next_tick + 1)\<close>
           unfolding real2_next_tick_def real_next_tick_def by auto
@@ -532,8 +562,8 @@ affirm unfolding \<Delta>growth_def real_next_tick_def apply auto
         using kk9 apply blast
         using kb2 by fastforce
 
-      have Iv6: \<open>if zeroForOne then reserve_change L next_price price = (amountIn, amountOut) + reserve_change L pr price
-                          else reserve_change L price next_price = reserve_change L price pr + (amountOut, amountIn)\<close>
+      have Iv6: \<open>if zeroForOne then reserve_change' L next_price price = (amountIn, amountOut) + reserve_change' L pr price
+                          else reserve_change' L price next_price = reserve_change' L price pr + (amountOut, amountIn)\<close>
         apply auto
         apply (smt (verit, best) add.commute kk6 p2 p3 price_of_L0 reserve_change_add_left the_\<phi>(21))
         using p2 p3 reserve_change_add_right the_\<phi>(2) the_\<phi>(21) by presburger
@@ -549,36 +579,88 @@ affirm unfolding \<Delta>growth_def real_next_tick_def apply auto
     using the_\<phi>(16) apply fastforce
     using the_\<phi>(16) apply fastforce
     using the_\<phi>(16) apply fastforce
-    using the_\<phi>(16) by fastforce
-  ;; \<exists>amount_remaining', price', amount_calculated', proto_fee', i'
-  ;;
+    using the_\<phi>(16) by fastforce ;;
+    \<exists>amount_remaining', price', amount_calculated', proto_fee', i' ;;
+
+  set_pool_tick ($tick)
+  set_pool_price ($price) ;;
+
   if \<open>$liquidityStart \<noteq> $liquidity\<close> \<medium_left_bracket> set_pool_liquidity ( $liquidity ) \<medium_right_bracket>. \<medium_left_bracket> \<medium_right_bracket>.
       is \<open>pool _ _ _ (L i') _ _ _\<close> affirm by auto ;;
 
+  have \<open>zeroForOne \<Longrightarrow>
+    growth.map_fee0 (\<lambda>_. I_fee_growth_global (growth + fee_growth zeroForOne fee_factor L price price')) (gSum growth)
+      = gSum (growth + fee_growth zeroForOne fee_factor L price price')\<close>
+    apply (auto simp add: prod_eq_iff growth.map_fee0_def I_fee_growth_global_def growth.fee0_def)
+    by (metis fee_growth_is_0_when_zeroForOne growth.fee1_def the_\<phi>(1) the_\<phi>lemmata(6))
+
+  have proto_fee': \<open>proto_fee' =
+    (if 0 < fee_proto then ((if zeroForOne then fst else snd) (reserve_change zeroForOne L price price')) * fee_factor / real fee_proto else 0)\<close>
+    by (smt (verit) fee_factor_def split_def the_\<phi>(16) times_divide_eq_right)
+
+  have proto_fee'_LE0: \<open>0 \<le> proto_fee'\<close>
+    unfolding proto_fee' using \<open>0 < price\<close> fee_factor_GT_0 reserve_change'_LE_0' the_\<phi>(1) the_\<phi>(12) the_\<phi>lemmata(6) by force ;;
+
+  if \<open>$zeroForOne\<close> \<medium_left_bracket>
+    set_pool_fee_growth_0 ($fee_growth_global)
+    is \<open>pool _ _ _ _ (gSum (growth + fee_growth zeroForOne fee_factor L price price')) _ _\<close>
+    affirm by (auto simp add: prod_eq_iff growth.map_fee0_def I_fee_growth_global_def growth.fee0_def growth.fee1_def the_\<phi>(15)) (metis fee_growth_is_0_when_zeroForOne growth.fee1_def the_\<phi>(1) the_\<phi>(15) the_\<phi>(18)) ;;
+
+    if \<open>$protocolFee > 0\<close> \<medium_left_bracket> set_pool_protocal_fee_0 (\<open>fst (pool.protocal_fees _) + $protocolFee\<close>) \<medium_right_bracket>. \<medium_left_bracket> \<medium_right_bracket>. ;;
+
+   \<medium_right_bracket>. \<medium_left_bracket>
+    set_pool_fee_growth_1 ($fee_growth_global)
+    is \<open>pool _ _ _ _ (gSum (growth + fee_growth zeroForOne fee_factor L price price')) _ _\<close>
+    affirm by (auto simp add: prod_eq_iff growth.map_fee1_def I_fee_growth_global_def growth.fee0_def growth.fee1_def the_\<phi>(15)) (metis \<open>0 < price\<close> fee_growth_is_0_when_not_zeroForOne growth.fee0_def the_\<phi>(15) the_\<phi>(18))  ;;
+
+    if \<open>$protocolFee > 0\<close> \<medium_left_bracket> set_pool_protocal_fee_1 (\<open>snd (pool.protocal_fees _) + $protocolFee\<close>) \<medium_right_bracket>. \<medium_left_bracket> \<medium_right_bracket>. ;;
+
+  \<medium_right_bracket>.
+  is \<open>pool price' i' False (L i') (gSum (growth + fee_growth zeroForOne fee_factor L price price')) fee_protocol
+           (protocal_fees + \<Delta>protocal_fees fee_protocol zeroForOne L price price' fee_factor)\<close>
+  affirm apply (cases protocal_fees; auto simp add: \<Delta>protocal_fees_def fee_proto_def proto_fee' zero_prod_def)
+    using fee_proto_def proto_fee' proto_fee'_LE0 zero_prod_def apply fastforce
+    using fee_proto_def proto_fee' proto_fee'_LE0 zero_prod_def apply fastforce
+    using fee_proto_def proto_fee' proto_fee'_LE0 apply force
+    using fee_proto_def proto_fee' proto_fee'_LE0 by fastforce ;;
 
 
-thm \<phi>
-term I_fee_growth_global;;
-if \<open>$zeroForOne\<close> \<medium_left_bracket>
-  $fee_growth_global
+  ;; if \<open>$zeroForOne = $exactInput\<close>
+      \<medium_left_bracket> \<open>$amount_specified - $amount_remaining\<close>, $amount_calculated \<medium_right_bracket>.
+      \<medium_left_bracket> $amount_calculated, \<open>$amount_specified - $amount_remaining\<close> \<medium_right_bracket>. \<rightarrow> val amount0, amount1 ;;
+  
+  $amount0 is \<open>if zeroForOne then fst (reserve_change' L price' price) / (1 - fee)
+                    else - fst (reserve_change' L price price')\<close>
+  affirm by (auto; insert the_\<phi>(16), force) ;; \<rightarrow> val amount0
 
+  $amount1 is \<open>if zeroForOne then - snd (reserve_change' L price' price)
+                    else snd (reserve_change' L price price') / (1 - fee)\<close>
+  affirm by (auto; insert the_\<phi>(16), force) ;; \<rightarrow> val amount1
 
-  thm \<phi>
-  thm \<open>case _ of (a,b) \<Rightarrow> _\<close>
-  have \<open>amount_remaining' = 0 \<Longrightarrow>
-        if zeroForOne
-        then if 0 < amount_specified
-             then amount_specified * (1 - fee) = fst (reserve_change L price' price)
-             else amount_specified = - snd (reserve_change L price' price)
-        else if 0 < amount_specified
-             then amount_specified * (1 - fee) = snd (reserve_change L price price')
-             else amount_specified = - fst (reserve_change L price price')\<close>
-    using \<open>case _ of (a,b) \<Rightarrow> _\<close> by auto
-  ;;    require (
- (*TODO: break parathensis scope in multi statements*)
+  if \<open>$zeroForOne\<close> \<medium_left_bracket>
+    if \<open>$amount1 < 0\<close> \<medium_left_bracket> \<open>-$amount1\<close> \<medium_right_bracket>. \<medium_left_bracket> \<open>0 \<Ztypecolon> \<real>\<close> \<medium_right_bracket>.
+    is \<open>snd (reserve_change' L price' price)\<close>
+    affirm apply auto
+        apply (smt (verit) reserve_change'_LE_0' the_\<phi>(1) the_\<phi>(12) the_\<phi>lemmata(6))
+        using the_\<phi>(15) apply blast
+        using the_\<phi>(15) by force ;;
 
+    $amount0 is \<open>fst (reserve_change' L price' price) / (1 - fee)\<close>
+  \<medium_right_bracket>. \<medium_left_bracket>
+    if \<open>$amount0 < 0\<close> \<medium_left_bracket> \<open>-$amount0\<close> \<medium_right_bracket>. \<medium_left_bracket> \<open>0 \<Ztypecolon> \<real>\<close> \<medium_right_bracket>.
+    is \<open>fst (reserve_change' L price price')\<close>
+    affirm by (auto simp add: the_\<phi>(15)) (smt (verit) \<open>0 < price\<close> reserve_change'_LE_0' the_\<phi>(12) the_\<phi>(15) the_\<phi>lemmata(6)) ;;
 
-  thm get_slot0_unlock_\<phi>app
+    $amount1 is \<open>snd (reserve_change' L price price') / (1 - fee)\<close>
+  \<medium_right_bracket>. ;;
+
+  set_pool_unlock (\<open>True\<close>)
+  note [[ML_print_depth = 1000]]
+  \<medium_right_bracket> apply (auto simp add: \<phi>)
+    apply (smt (verit, best) \<open>(if zeroForOne = (0 < amount_specified) then amount_specified - amount_remaining' else amount_calculated') = (if zeroForOne then fst (reserve_change' L price' price) / (1 - fee) else - fst (reserve_change' L price price'))\<close> fee_range nonzero_divide_eq_eq the_\<phi>lemmata(8))
+    using \<open>(if zeroForOne = (0 < amount_specified) then amount_calculated' else amount_specified - amount_remaining') = (if zeroForOne then - snd (reserve_change' L price' price) else snd (reserve_change' L price price') / (1 - fee))\<close> the_\<phi>lemmata(8) apply force
+    using \<open>(if zeroForOne = (0 < amount_specified) then amount_calculated' else amount_specified - amount_remaining') = (if zeroForOne then - snd (reserve_change' L price' price) else snd (reserve_change' L price price') / (1 - fee))\<close> \<open>0 \<noteq> amount_specified \<and> 0 < price_limit\<close> the_\<phi>lemmata(8) apply force
+    using \<open>(if zeroForOne = (0 < amount_specified) then amount_specified - amount_remaining' else amount_calculated') = (if zeroForOne then fst (reserve_change' L price' price) / (1 - fee) else - fst (reserve_change' L price price'))\<close> the_\<phi>lemmata(8) by force .
 
 end
 
